more wibbles

Core/Infer/Global.lean
@@ -12,22 +12,24 @@ def GlobalEnv.wf_globals : GlobalEnv -> Option Unit
 | .cons (.data (n := n) x k ctors) G => do
   wf_globals G
   if (lookup x G).isNone then
-  let mctors' : Fun.Vec (Option Unit) n := λ i => spine_kinding (.data (n := 0) x k #𝓋[] :: G) (ctors.get_elem i).snd
+  let mctors' : Fun.Vec (Option Unit) n :=
+    λ i => spine_kinding (.data (n := 0) x k #𝓋[] :: G) (.data .cls) (ctors[i].fst) (ctors[i].snd)
   let _ <- mctors'.to.seq
 | .cons (.openm x spTy) G => do
   wf_globals G
   if (lookup x G).isNone
-  then spine_kinding G spTy
+  then spine_kinding G .openm x spTy
   else none
 | .cons (.octor x spTy) G => do
   wf_globals G
   if (lookup x G).isNone
-  then spine_kinding G spTy
+  then spine_kinding G (.data .opn) x spTy
   else none
 | .cons (.defn x T t) G => do
   wf_globals G
   let T' <- t.infer_type G [] []
-  let _ <- T.infer_kind G []
+  let Tk <- T.infer_kind G []
+  let _ <- Tk.base_kind
   if T == T' && (lookup x G).isNone then return () else none
 | .cons (.inst x p t) G => do
   wf_globals G
@@ -43,4 +45,14 @@ def GlobalEnv.wf_globals : GlobalEnv -> Option Unit
   wf_globals G
   if (lookup x G).isNone
   then return () else none
+
+
+def GlobalEnv.check_open_exhaustive : GlobalEnv -> Option Unit
+| _ => none
+
+-- For each method,
+-- collect the instances of the method
+-- collect the patterns for each instance
+-- check that the patterns together are exhaustive
+
 end Core
