Core/Infer/GlobalSound.lean
@@ -8,24 +8,73 @@ import Core.Global
 namespace Core
 
 theorem wf_global_sound :
-  ⊢ G ->
-  Globals.wf_globals G = some () := by
-intro wf
-induction G <;> simp at *
-case cons hdg tlg ih =>
-  cases wf; case _ wfg wftlg =>
-  replace ih := ih wfg
-  cases hdg <;> simp at *
-  case data =>
-    rw[Option.bind_eq_some_iff]; exists ()
-    constructor; assumption
-    rw[Option.bind_eq_some_iff];
+  GlobalEnv.wf_globals G = some () ->
+  ⊢ G
+:= by
+intro h
+fun_induction GlobalEnv.wf_globals <;> simp at *
+case _ =>  -- empty
+  apply ListGlobalWf.nil
 
+case _ ih => -- ctors
+  rw[Option.bind_eq_some_iff] at h; rcases h with ⟨h1, h2, h⟩
+  simp at h
+  apply ListGlobalWf.cons
+  · sorry
+  · apply ih h2
+
+case _ ih =>  -- openm
+  rw[Option.bind_eq_some_iff] at h; rcases h with ⟨h1, h2, h⟩
+  simp at h
+  apply ListGlobalWf.cons
+  · sorry
+  · apply ih h2
+
+case _ ih =>  -- octor
+  rw[Option.bind_eq_some_iff] at h; rcases h with ⟨h1, h2, h⟩
+  simp at h; rcases h with ⟨e, h⟩
+  apply ListGlobalWf.cons
+  · apply GlobalWf.octor
     sorry
-  case opent =>  sorry
-  case openm => sorry
-  case defn => sorry
-  case inst => sorry
-  case instty => sorry
+    apply e
+  · apply ih h2
+
+case _ ih => -- defn
+  rw[Option.bind_eq_some_iff] at h; rcases h with ⟨h1, h2, h⟩
+  rw[Option.bind_eq_some_iff] at h; rcases h with ⟨h3, h4, h⟩
+  rw[Option.bind_eq_some_iff] at h; rcases h with ⟨h5, h6, h⟩
+  rw[Option.bind_eq_some_iff] at h; rcases h with ⟨h7, h8, h⟩
+  simp at h; rcases h with ⟨e1, h⟩; subst e1
+  apply ListGlobalWf.cons
+  · apply GlobalWf.defn
+    · replace h8 := Kind.base_kind_sound _ h8; subst h5
+      replace h6 := infer_kind_sound h6; apply h6
+    · replace h4 := infer_type_sound (ih h2) h4; apply h4
+    · apply h
+  · apply ih h2
+
+case _ ih => -- inst
+  rw[Option.bind_eq_some_iff] at h; rcases h with ⟨h1, h2, h⟩
+  split at h
+  · rw[Option.bind_eq_some_iff] at h; rcases h with ⟨h3, h4, h⟩
+    rw[Option.bind_eq_some_iff] at h; rcases h with ⟨h5, h6, h⟩
+    simp at h
+    apply ListGlobalWf.cons
+    · sorry
+    · apply ih h2
+  · cases h
+
+case _ ih => -- odata
+  rw[Option.bind_eq_some_iff] at h; rcases h with ⟨h1, h2, h⟩
+  simp at h
+  apply ListGlobalWf.cons
+  · apply GlobalWf.odata h
+  · apply ih h2
+
+
+
+theorem open_exhaustive_sound {G : GlobalEnv} :
+  G.check_open_exhaustive = some () ->
+  OpenExhaustive G := by sorry
 
 end Core
